	\solu{We will rename the sequence and call it $ \{s_i\} $, with $ s_0=x\in \Z $. Now let, \[s_i = \frac{a_ix+b_i}{c_ix+d_i}\]
		
	At the beginning we have $ a_0=d_0=1, b_0=c_0=0 $. It is easy to prove that \[ a_{i+1}+c_{i+1} = 2(a_i+c_i) \]\[ b_{i+1}+d_{i+1} = 2(b_i+d_i) \]
	So it follows that \[ a_i+c_i = 2^i = b_i+d_i \]
	Also, by induction (which is easy to prove), we have \[a_i - b_i = d_i - c_i = 1\]
	
	Suppose for some $ k $, $ s_k=2014 $. So, 
	\begin{align}
	&\frac{a_kx+b_k}{c_kx+d_k}=2014\\[1em]
	\implies x&=\frac{2014d_k-b_k}{a_k-2014c_k}=\frac{2015d_k-2^k}{2^k-2015c_k}\\[1em]
	&=\frac{2015(d_k-c_k)}{2^k-2015c_k}-1
	\end{align}
	
	But $ \gcd(2015, 2^k-2015c_k)=1 $, which implies $ 2^k-2015-c_k=1 $. Solving for $ k $ with CRT gives us $ 60|k $. 
	
	Now we have to prove that there is a sequence with $ s_{60} = 2014 $. Solving (1), $ s_0=2014 $, and,
	\begin{align*}
	a_{60}&= \frac{2014\cdot 2^{60}+1}{2015} &b_{60} &=\frac{2014\cdot 2^{60}-2014}{2015}\\[1em]
	c_{60}&= \frac{2^{60}-1}{2015} &d_{60} &=\frac{2^{60}+2014}{2015}
	\end{align*}
	
	We show that we can make $ (a_{60}, c_{60}) $ from $ (a_0, c_0)=(1, 0) $. We prove it by induction, that $ (a_k, c_k) $ can take any form $ (2^k-i, i) $ with $ i\in\{0, 1, \dots 2^k-1\} $.}